Some modifications of sequence files

Seqs.i.dfy
@@ -1,44 +1,44 @@
 module Collections__Seqs_i {
 
-lemma SeqAdditionIsAssociative<T>(a:seq<T>, b:seq<T>, c:seq<T>)
+lemma lemma_seq_addition_is_associative<T>(a:seq<T>, b:seq<T>, c:seq<T>)
 // explains associative property of sequences in addition
   ensures a+(b+c) == (a+b)+c;
 {
 }
 
-predicate ItemAtPositionInSeq<T>(s:seq<T>, v:T, idx:int)
+predicate item_at_position_in_sequence<T>(s:seq<T>, v:T, idx:int)
 // defines if the element is at a specific position in the sequence
 {
   0 <= idx < |s| && s[idx] == v
 }
 
-lemma Lemma_ItemInSeqAtASomePosition<T>(s:seq<T>, v:T)
+lemma lemma_item_at_position_in_sequence<T>(s:seq<T>, v:T)
 // if there is an element at a certain index, then that index exists
   requires v in s
-  ensures exists idx :: ItemAtPositionInSeq(s, v, idx)
+  ensures exists idx :: item_at_position_in_sequence(s, v, idx)
 {
   var idx :| 0 <= idx < |s| && s[idx] == v;
-  assert ItemAtPositionInSeq(s, v, idx);
+  assert item_at_position_in_sequence(s, v, idx);
 }
 
-function FindIndexInSeq<T>(s:seq<T>, v:T):int
+function find_index_in_sequence<T>(s:seq<T>, v:T):int
 /* finds the index of a certain value in the sequence, if it exists. Returns
 the index, or -1 if the value is not included in the sequence */
-  ensures var idx := FindIndexInSeq(s, v);
+  ensures var idx := find_index_in_sequence(s, v);
           if idx >= 0 then
             idx < |s| && s[idx] == v
           else
             v !in s
 {
   if v in s then
-    Lemma_ItemInSeqAtASomePosition(s, v);
-    var idx :| ItemAtPositionInSeq(s, v, idx);
+    lemma_item_at_position_in_sequence(s, v);
+    var idx :| item_at_position_in_sequence(s, v, idx);
     idx
   else
     -1
 }
 
-lemma Lemma_IdenticalSingletonSequencesHaveIdenticalElement<T>(x:T, y:T)
+lemma lemma_identical_seq_singletons_have_itentical_elements<T>(x:T, y:T)
 // two identical sequences of length 1 have the same elements
   requires [x] == [y]
   ensures  x == y
@@ -70,75 +70,78 @@ original sequence except for the last element */
 //////////////////////////////////////////////////////////
 //  Combining sequences of sequences
 //////////////////////////////////////////////////////////
-function SeqCat<T>(seqs:seq<seq<T>>) : seq<T>
-// concatenates a sequence of sequences into a single sequence
+function seq_concat<T>(seqs:seq<seq<T>>) : seq<T>
+/* concatenates a sequence of sequences into a single sequence. 
+Works by adding elements in order from first to last */
   decreases |seqs|
 {
   if |seqs| == 0 then []
-  else seqs[0] + SeqCat(seqs[1..])
+  else seqs[0] + seq_concat(seqs[1..])
 }
 
-function SeqCatRev<T>(seqs:seq<seq<T>>) : seq<T>
-// concatenates the sequence in reverse and returns the resulting sequence  
+function seq_concat_reverse<T>(seqs:seq<seq<T>>) : seq<T>
+/* concatenates the sequence of sequences into a single sequence. 
+works by adding elements from last to first */
   decreases |seqs|
 {
   if |seqs| == 0 then []
-  else SeqCatRev(all_but_last(seqs)) + last(seqs)
+  else seq_concat_reverse(all_but_last(seqs)) + last(seqs)
 }
 
-lemma lemma_SeqCat_adds<T>(A:seq<seq<T>>, B:seq<seq<T>>)
+lemma lemma_seq_concat_adds<T>(A:seq<seq<T>>, B:seq<seq<T>>)
 /* concatenating two sequences of sequences is equivalent to concatenating
 each sequence of sequences seperately, and then concatenating the two resulting 
 sequences together */
-  ensures SeqCat(A + B) == SeqCat(A) + SeqCat(B)
+  ensures seq_concat(A + B) == seq_concat(A) + seq_concat(B)
 {
   if |A| == 0 {
     assert A+B == B;
   } else {
     calc == {
-      SeqCat(A + B);
+      seq_concat(A + B);
         { assert (A + B)[0] == A[0];  assert (A + B)[1..] == A[1..] + B; }
-      A[0] + SeqCat(A[1..] + B);
-      A[0] + SeqCat(A[1..]) + SeqCat(B);
-      SeqCat(A) + SeqCat(B);
+      A[0] + seq_concat(A[1..] + B);
+      A[0] + seq_concat(A[1..]) + seq_concat(B);
+      seq_concat(A) + seq_concat(B);
     }
   }
 }
 
-lemma lemma_SeqCatRev_adds<T>(A:seq<seq<T>>, B:seq<seq<T>>)
+lemma lemma_seq_concat_reverse_adds<T>(A:seq<seq<T>>, B:seq<seq<T>>)
 /* concatenating two reversed sequences of sequences is the same as reversing two 
 sequences of sequences and then adding the two resulting sequences together */
-  ensures SeqCatRev(A + B) == SeqCatRev(A) + SeqCatRev(B)
+  ensures seq_concat_reverse(A + B) == seq_concat_reverse(A) + seq_concat_reverse(B)
 {
   if |B| == 0 {
-    assert SeqCatRev(B) == [];
+    assert seq_concat_reverse(B) == [];
     assert A+B == A;
   } else {
     calc == {
-      SeqCatRev(A + B);
+      seq_concat_reverse(A + B);
         { assert last(A + B) == last(B);  assert all_but_last(A + B) == A + all_but_last(B); }
-      SeqCatRev(A + all_but_last(B)) + last(B);
-      SeqCatRev(A) + SeqCatRev(all_but_last(B)) + last(B);
-      SeqCatRev(A) + SeqCatRev(B);
+      seq_concat_reverse(A + all_but_last(B)) + last(B);
+      seq_concat_reverse(A) + seq_concat_reverse(all_but_last(B)) + last(B);
+      seq_concat_reverse(A) + seq_concat_reverse(B);
     }
   }
 }
 
-lemma lemma_SeqCat_equivalent<T>(seqs:seq<seq<T>>)
-// 
-  ensures SeqCat(seqs) == SeqCatRev(seqs)
+lemma lemma_seq_concat_and_seq_concat_reverse_are_equivalent<T>(seqs:seq<seq<T>>)
+/* both methods of concatenating sequence (starting from front v. starting from back)
+result in the same sequence */
+  ensures seq_concat(seqs) == seq_concat_reverse(seqs)
 {
   if |seqs| == 0 {
   } else {
     calc == {
-      SeqCatRev(seqs);
-      SeqCatRev(all_but_last(seqs)) + last(seqs);
-        { lemma_SeqCat_equivalent(all_but_last(seqs)); }
-      SeqCat(all_but_last(seqs)) + last(seqs);
-      SeqCat(all_but_last(seqs)) + SeqCat([last(seqs)]);
-        { lemma_SeqCat_adds(all_but_last(seqs), [last(seqs)]); 
+      seq_concat_reverse(seqs);
+      seq_concat_reverse(all_but_last(seqs)) + last(seqs);
+        { lemma_seq_concat_and_seq_concat_reverse_are_equivalent(all_but_last(seqs)); }
+      seq_concat(all_but_last(seqs)) + last(seqs);
+      seq_concat(all_but_last(seqs)) + seq_concat([last(seqs)]);
+        { lemma_seq_concat_adds(all_but_last(seqs), [last(seqs)]); 
       assert seqs == all_but_last(seqs) + [last(seqs)]; }
-      SeqCat(seqs);
+      seq_concat(seqs);
     }
   }
 }
